Port x86's pregs to the Registerfile representation
This makes all preg accesses typed, so a large number of proofs must be
adjusted. Some other details change as well due to typing; for example,
trying to execute x86_64 instructions in 32-bit mode is an error.

x86/Asm.v
@@ -38,10 +38,31 @@ Proof. decide equality. Defined.
 Lemma freg_eq: forall (x y: freg), {x=y} + {x<>y}.
 Proof. decide equality. Defined.
 
+Definition ireg_index (i: ireg): Z :=
+  2 + 2 * match i with
+  | RAX =>  0 | RBX =>  1 | RCX =>  2 | RDX =>  3
+  | RSI =>  4 | RDI =>  5 | RBP =>  6 | RSP =>  7
+  | R8  =>  8 | R9  =>  9 | R10 => 10 | R11 => 11
+  | R12 => 12 | R13 => 13 | R14 => 14 | R15 => 15
+  end.
+
+Definition freg_index (f: freg): Z :=
+  34 + 2 * match f with
+  | XMM0  =>  0 | XMM1  =>  1 | XMM2  =>  2 | XMM3  =>  3
+  | XMM4  =>  4 | XMM5  =>  5 | XMM6  =>  6 | XMM7  =>  7
+  | XMM8  =>  8 | XMM9  =>  9 | XMM10 => 10 | XMM11 => 11
+  | XMM12 => 12 | XMM13 => 13 | XMM14 => 14 | XMM15 => 15
+  end.
+
 (** Bits of the flags register. *)
 
 Inductive crbit: Type :=
   | ZF | CF | PF | SF | OF.
+
+Definition crbit_index (c: crbit): Z :=
+  66 + 2 * match c with
+  | ZF => 0 | CF => 1 | PF => 2 | SF => 3 | OF => 4
+  end.
 
 (** All registers modeled here. *)
 
@@ -308,18 +329,165 @@ Definition program := AST.program fundef unit.
 Lemma preg_eq: forall (x y: preg), {x=y} + {x<>y}.
 Proof. decide equality. apply ireg_eq. apply freg_eq. decide equality. Defined.
 
-Module PregEq.
-  Definition t := preg.
-  Definition eq := preg_eq.
-End PregEq.
+Definition preg_index (p: preg): Z :=
+  match p with
+  | IR i => ireg_index i
+  | FR f => freg_index f
+  | CR c => crbit_index c
+  | PC   => 76
+  | ST0  => 78
+  | RA   => 80
+  end.
 
-Module Pregmap := EMap(PregEq).
+Lemma preg_index_bounds:
+  forall p: preg,
+  match p with
+  | IR _ =>  0 < preg_index p /\ preg_index p <= 32
+  | FR _ => 33 < preg_index p /\ preg_index p <= 64
+  | CR _ => 65 < preg_index p /\ preg_index p <= 74
+  | _    => 75 < preg_index p
+  end.
+Proof.
+  destruct p; unfold preg_index; try omega.
+  destruct i; unfold ireg_index; omega.
+  destruct f; unfold freg_index; omega.
+  destruct c; unfold crbit_index; omega.
+Qed.
 
-Definition regset := Pregmap.t val.
+Module Preg <: REGISTER_MODEL.
+
+  Definition reg := preg.
+  Definition eq_dec := preg_eq.
+
+  Definition type p :=
+    match p with
+    | IR _    => if Archi.ptr64 then Tany64 else Tany32
+    | PC | RA => if Archi.ptr64 then Tany64 else Tany32
+    | FR _    => Tany64
+    | CR _    => Tany32
+    | ST0     => Tany64
+    end.
+
+  Definition quantity_of p :=
+    match p with
+    | IR _    => if Archi.ptr64 then Q64 else Q32
+    | PC | RA => if Archi.ptr64 then Q64 else Q32
+    | FR _    => Q64
+    | CR _    => Q32
+    | ST0     => Q64
+    end.
+
+  Definition chunk_of p :=
+    match p with
+    | IR _    => if Archi.ptr64 then Many64 else Many32
+    | PC | RA => if Archi.ptr64 then Many64 else Many32
+    | FR _    => Many64
+    | CR _    => Many32
+    | ST0     => Many64
+    end.
+
+  Lemma type_cases: forall r, type r = Tany32 \/ type r = Tany64.
+  Proof.
+    destruct r; simpl; auto.
+  Qed.
+
+  Definition ofs (r: preg): Z :=
+    preg_index r.
+
+  (* A register's address: The index of its first byte. *)
+  Definition addr (r: preg): Z :=
+    preg_index r * 4.
+
+  (* The address one byte past the end of register [r]. The next nonoverlapping
+     register may start here. *)
+  Definition next_addr (r: preg): Z := addr r + AST.typesize (type r).
+
+  Remark addr_pos: forall p, addr p > 0.
+  Proof.
+    intros. unfold addr.
+    destruct p; simpl; try omega.
+    destruct i; simpl; omega.
+    destruct f; simpl; omega.
+    destruct c; simpl; omega.
+  Qed.
+
+  Lemma addr_compat: forall p, FragBlock.addr (ofs p) = addr p.
+  Proof.
+    reflexivity.
+  Qed.
+
+  Lemma size_compat:
+    forall p,
+    AST.typesize (type p) = FragBlock.quantity_size (quantity_of p).
+  Proof.
+    intros. unfold quantity_of.
+    destruct p; simpl; auto.
+  Qed.
+
+  Lemma next_addr_compat: forall p, FragBlock.next_addr (ofs p) (quantity_of p) = next_addr p.
+  Proof.
+    unfold next_addr, addr, ofs, FragBlock.next_addr, FragBlock.addr; intros.
+    rewrite size_compat. auto.
+  Qed.
+
+  Lemma quantity_of_compat:
+    forall p,
+    quantity_of p = quantity_of_typ (type p).
+  Proof.
+    destruct p; simpl; destruct Archi.ptr64; try destruct i; reflexivity.
+  Qed.
+
+  Lemma chunk_of_reg_compat:
+    forall p,
+    chunk_of p = chunk_of_quantity (quantity_of p).
+  Proof.
+    destruct p; simpl; destruct Archi.ptr64; try destruct i; reflexivity.
+  Qed.
+
+  Lemma chunk_of_reg_type:
+    forall p,
+    chunk_of p = chunk_of_type (type p).
+  Proof.
+    destruct p; simpl; destruct Archi.ptr64; try destruct i; reflexivity.
+  Qed.
+
+  Lemma diff_outside_interval:
+    forall r s, r <> s -> next_addr r <= addr s \/ next_addr s <= addr r.
+  Proof.
+    intros.
+    unfold next_addr, addr.
+    assert (TS: forall p, AST.typesize (type p) = 4 \/ AST.typesize (type p) = 8).
+    { intro p. destruct (type_cases p) as [T | T]; rewrite T; auto. }
+    generalize (preg_index_bounds r), (preg_index_bounds s); intros RB SB.
+    destruct r eqn:R, s eqn:S;
+      try congruence;
+      try (destruct (TS r), (TS s); subst; omega);
+      simpl AST.typesize;
+      try (destruct Archi.ptr64; simpl; omega).
+    - (* two iregs *)
+      destruct Archi.ptr64; simpl; destruct i, i0; simpl; try omega; congruence.
+    - (* two fregs *)
+      destruct f, f0; simpl; try omega; congruence.
+    - (* two crbits *)
+      destruct Archi.ptr64; destruct c, c0; simpl; try omega; congruence.
+  Qed.
+
+End Preg.
+
+Lemma pc_type: subtype Tptr (Preg.type PC) = true.
+Proof.
+  unfold Tptr. simpl Preg.type. destruct Archi.ptr64; auto.
+Qed.
+
+Module Pregmap := Regfile(Preg).
+
+Definition regset := Pregmap.t.
 Definition genv := Genv.t fundef unit.
 
-Notation "a # b" := (a b) (at level 1, only parsing) : asm.
+Notation "a # b" := (Pregmap.get b a) (at level 1, only parsing) : asm.
 Notation "a # b <- c" := (Pregmap.set b c a) (at level 1, b at next level) : asm.
+
+Definition pregmap_read (rs: regset) := fun r => Pregmap.get r rs.
 
 Open Scope asm.
 
@@ -328,8 +496,25 @@ Open Scope asm.
 Fixpoint undef_regs (l: list preg) (rs: regset) : regset :=
   match l with
   | nil => rs
-  | r :: l' => undef_regs l' (rs#r <- Vundef)
+  | r :: l' => (undef_regs l' rs)#r <- Vundef
   end.
+
+Lemma undef_regs_other:
+  forall r rl rs, ~In r rl -> (undef_regs rl rs) # r = rs # r.
+Proof.
+  induction rl; simpl; intros. auto. rewrite Pregmap.gso. apply IHrl. intuition. intuition.
+Qed.
+
+Lemma undef_regs_same:
+  forall r rl rs, In r rl -> (undef_regs rl rs) # r = Vundef.
+Proof.
+  induction rl; simpl; intros. tauto.
+  destruct H.
+  - subst a. rewrite Pregmap.gss. destruct (Preg.chunk_of r); auto.
+  - destruct (Preg.eq_dec r a).
+    + subst a. rewrite Pregmap.gss. destruct (Preg.chunk_of r); auto.
+    + rewrite Pregmap.gso; auto.
+Qed.
 
 (** Assigning a register pair *)
 
@@ -389,14 +574,14 @@ Definition eval_addrmode32 (a: addrmode) (rs: regset) : val :=
   let '(Addrmode base ofs const) := a in
   Val.add  (match base with
              | None => Vint Int.zero
-             | Some r => rs r
+             | Some r => rs # r
             end)
   (Val.add (match ofs with
              | None => Vint Int.zero
              | Some(r, sc) =>
                 if zeq sc 1
-                then rs r
-                else Val.mul (rs r) (Vint (Int.repr sc))
+                then rs # r
+                else Val.mul (rs # r) (Vint (Int.repr sc))
              end)
            (match const with
             | inl ofs => Vint (Int.repr ofs)
@@ -407,14 +592,14 @@ Definition eval_addrmode64 (a: addrmode) (rs: regset) : val :=
   let '(Addrmode base ofs const) := a in
   Val.addl (match base with
              | None => Vlong Int64.zero
-             | Some r => rs r
+             | Some r => rs # r
             end)
   (Val.addl (match ofs with
              | None => Vlong Int64.zero
              | Some(r, sc) =>
                 if zeq sc 1
-                then rs r
-                else Val.mull (rs r) (Vlong (Int64.repr sc))
+                then rs # r
+                else Val.mull (rs # r) (Vlong (Int64.repr sc))
              end)
            (match const with
             | inl ofs => Vlong (Int64.repr ofs)
@@ -484,62 +669,62 @@ Definition compare_floats32 (vx vy: val) (rs: regset) : regset :=
 Definition eval_testcond (c: testcond) (rs: regset) : option bool :=
   match c with
   | Cond_e =>
-      match rs ZF with
+      match rs # ZF with
       | Vint n => Some (Int.eq n Int.one)
       | _ => None
       end
   | Cond_ne =>
-      match rs ZF with
+      match rs # ZF with
       | Vint n => Some (Int.eq n Int.zero)
       | _ => None
       end
   | Cond_b =>
-      match rs CF with
+      match rs # CF with
       | Vint n => Some (Int.eq n Int.one)
       | _ => None
       end
   | Cond_be =>
-      match rs CF, rs ZF with
+      match rs # CF, rs # ZF with
       | Vint c, Vint z => Some (Int.eq c Int.one || Int.eq z Int.one)
       | _, _ => None
       end
   | Cond_ae =>
-      match rs CF with
+      match rs # CF with
       | Vint n => Some (Int.eq n Int.zero)
       | _ => None
       end
   | Cond_a =>
-      match rs CF, rs ZF with
+      match rs # CF, rs # ZF with
       | Vint c, Vint z => Some (Int.eq c Int.zero && Int.eq z Int.zero)
       | _, _ => None
       end
   | Cond_l =>
-      match rs OF, rs SF with
+      match rs # OF, rs # SF with
       | Vint o, Vint s => Some (Int.eq (Int.xor o s) Int.one)
       | _, _ => None
       end
   | Cond_le =>
-      match rs OF, rs SF, rs ZF with
+      match rs # OF, rs # SF, rs # ZF with
       | Vint o, Vint s, Vint z => Some (Int.eq (Int.xor o s) Int.one || Int.eq z Int.one)
       | _, _, _ => None
       end
   | Cond_ge =>
-      match rs OF, rs SF with
+      match rs # OF, rs # SF with
       | Vint o, Vint s => Some (Int.eq (Int.xor o s) Int.zero)
       | _, _ => None
       end
   | Cond_g =>
-      match rs OF, rs SF, rs ZF with
+      match rs # OF, rs # SF, rs # ZF with
       | Vint o, Vint s, Vint z => Some (Int.eq (Int.xor o s) Int.zero && Int.eq z Int.zero)
       | _, _, _ => None
       end
   | Cond_p =>
-      match rs PF with
+      match rs # PF with
       | Vint n => Some (Int.eq n Int.one)
       | _ => None
       end
   | Cond_np =>
-      match rs PF with
+      match rs # PF with
       | Vint n => Some (Int.eq n Int.zero)
       | _ => None
       end
@@ -588,7 +773,7 @@ Definition exec_load (chunk: memory_chunk) (m: mem)
 Definition exec_store (chunk: memory_chunk) (m: mem)
                       (a: addrmode) (rs: regset) (r1: preg)
                       (destroyed: list preg) :=
-  match Mem.storev chunk m (eval_addrmode a rs) (rs r1) with
+  match Mem.storev chunk m (eval_addrmode a rs) (rs # r1) with
   | Some m' => Next (nextinstr_nf (undef_regs destroyed rs)) m'
   | None => Stuck
   end.
@@ -616,7 +801,7 @@ Definition exec_instr (f: function) (i: instruction) (rs: regset) (m: mem) : out
   match i with
   (** Moves *)
   | Pmov_rr rd r1 =>
-      Next (nextinstr (rs#rd <- (rs r1))) m
+      Next (nextinstr (rs#rd <- (rs # r1))) m
   | Pmovl_ri rd n =>
       Next (nextinstr_nf (rs#rd <- (Vint n))) m
   | Pmovq_ri rd n =>
@@ -632,7 +817,7 @@ Definition exec_instr (f: function) (i: instruction) (rs: regset) (m: mem) : out
   | Pmovq_mr a r1 =>
       exec_store Mint64 m a rs r1 nil
   | Pmovsd_ff rd r1 =>
-      Next (nextinstr (rs#rd <- (rs r1))) m
+      Next (nextinstr (rs#rd <- (rs # r1))) m
   | Pmovsd_fi rd n =>
       Next (nextinstr (rs#rd <- (Vfloat n))) m
   | Pmovsd_fm rd a =>
@@ -854,21 +1039,21 @@ Definition exec_instr (f: function) (i: instruction) (rs: regset) (m: mem) : out
   | Prorq_ri rd n =>
       Next (nextinstr_nf (rs#rd <- (Val.rorl rs#rd (Vint n)))) m
   | Pcmpl_rr r1 r2 =>
-      Next (nextinstr (compare_ints (rs r1) (rs r2) rs m)) m
+      Next (nextinstr (compare_ints (rs # r1) (rs # r2) rs m)) m
   | Pcmpq_rr r1 r2 =>
-      Next (nextinstr (compare_longs (rs r1) (rs r2) rs m)) m
+      Next (nextinstr (compare_longs (rs # r1) (rs # r2) rs m)) m
   | Pcmpl_ri r1 n =>
-      Next (nextinstr (compare_ints (rs r1) (Vint n) rs m)) m
+      Next (nextinstr (compare_ints (rs # r1) (Vint n) rs m)) m
   | Pcmpq_ri r1 n =>
-      Next (nextinstr (compare_longs (rs r1) (Vlong n) rs m)) m
+      Next (nextinstr (compare_longs (rs # r1) (Vlong n) rs m)) m
   | Ptestl_rr r1 r2 =>
-      Next (nextinstr (compare_ints (Val.and (rs r1) (rs r2)) Vzero rs m)) m
+      Next (nextinstr (compare_ints (Val.and (rs # r1) (rs # r2)) Vzero rs m)) m
   | Ptestq_rr r1 r2 =>
-      Next (nextinstr (compare_longs (Val.andl (rs r1) (rs r2)) (Vlong Int64.zero) rs m)) m
+      Next (nextinstr (compare_longs (Val.andl (rs # r1) (rs # r2)) (Vlong Int64.zero) rs m)) m
   | Ptestl_ri r1 n =>
-      Next (nextinstr (compare_ints (Val.and (rs r1) (Vint n)) Vzero rs m)) m
+      Next (nextinstr (compare_ints (Val.and (rs # r1) (Vint n)) Vzero rs m)) m
   | Ptestq_ri r1 n =>
-      Next (nextinstr (compare_longs (Val.andl (rs r1) (Vlong n)) (Vlong Int64.zero) rs m)) m
+      Next (nextinstr (compare_longs (Val.andl (rs # r1) (Vlong n)) (Vlong Int64.zero) rs m)) m
   | Pcmov c rd r1 =>
       match eval_testcond c rs with
       | Some true => Next (nextinstr (rs#rd <- (rs#r1))) m
@@ -891,7 +1076,7 @@ Definition exec_instr (f: function) (i: instruction) (rs: regset) (m: mem) : out
   | Pabsd rd =>
       Next (nextinstr (rs#rd <- (Val.absf rs#rd))) m
   | Pcomisd_ff r1 r2 =>
-      Next (nextinstr (compare_floats (rs r1) (rs r2) rs)) m
+      Next (nextinstr (compare_floats (rs # r1) (rs # r2) rs)) m
   | Pxorpd_f rd =>
       Next (nextinstr_nf (rs#rd <- (Vfloat Float.zero))) m
   (** Arithmetic operations over single-precision floats *)
@@ -908,7 +1093,7 @@ Definition exec_instr (f: function) (i: instruction) (rs: regset) (m: mem) : out
   | Pabss rd =>
       Next (nextinstr (rs#rd <- (Val.absfs rs#rd))) m
   | Pcomiss_ff r1 r2 =>
-      Next (nextinstr (compare_floats32 (rs r1) (rs r2) rs)) m
+      Next (nextinstr (compare_floats32 (rs # r1) (rs # r2) rs)) m
   | Pxorps_f rd =>
       Next (nextinstr_nf (rs#rd <- (Vsingle Float32.zero))) m
   (** Branches and calls *)
@@ -917,7 +1102,7 @@ Definition exec_instr (f: function) (i: instruction) (rs: regset) (m: mem) : out
   | Pjmp_s id sg =>
       Next (rs#PC <- (Genv.symbol_address ge id Ptrofs.zero)) m
   | Pjmp_r r sg =>
-      Next (rs#PC <- (rs r)) m
+      Next (rs#PC <- (rs # r)) m
   | Pjcc cond lbl =>
       match eval_testcond cond rs with
       | Some true => goto_label f lbl rs m
@@ -942,7 +1127,7 @@ Definition exec_instr (f: function) (i: instruction) (rs: regset) (m: mem) : out
   | Pcall_s id sg =>
       Next (rs#RA <- (Val.offset_ptr rs#PC Ptrofs.one) #PC <- (Genv.symbol_address ge id Ptrofs.zero)) m
   | Pcall_r r sg =>
-      Next (rs#RA <- (Val.offset_ptr rs#PC Ptrofs.one) #PC <- (rs r)) m
+      Next (rs#RA <- (Val.offset_ptr rs#PC Ptrofs.one) #PC <- (rs # r)) m
   | Pret =>
       Next (rs#PC <- (rs#RA)) m
   (** Saving and restoring registers *)
@@ -1073,12 +1258,41 @@ Definition preg_of (r: mreg) : preg :=
 
 (** Undefine all registers except SP and callee-save registers *)
 
-Definition undef_caller_save_regs (rs: regset) : regset :=
+Definition undef_caller_save_regs_spec (rs: preg -> val) : preg -> val :=
   fun r =>
     if preg_eq r SP
     || In_dec preg_eq r (List.map preg_of (List.filter is_callee_save all_mregs))
     then rs r
     else Vundef.
+
+Definition pregs_destroyed_at_call :=
+  PC :: ST0 :: CR ZF :: CR CF :: CR PF :: CR SF :: CR OF :: RA
+     :: (map preg_of (filter (fun m => negb (is_callee_save m)) all_mregs)).
+
+Lemma pregs_destroyed_at_call_correct:
+  forall r,
+  preg_eq r SP
+  || In_dec preg_eq r (List.map preg_of (List.filter is_callee_save all_mregs))
+  =
+  negb (In_dec preg_eq r pregs_destroyed_at_call).
+Proof.
+  intros.
+  destruct r as [|x|x| |x|]; try destruct x; auto.
+Qed.
+
+Definition undef_caller_save_regs (rs: regset) : regset :=
+  undef_regs pregs_destroyed_at_call rs.
+
+Lemma undef_caller_save_regs_correct:
+  forall rs r,
+  (undef_caller_save_regs rs) # r = undef_caller_save_regs_spec (fun r' => rs # r) r.
+Proof.
+  intros. unfold undef_caller_save_regs, undef_caller_save_regs_spec.
+  rewrite pregs_destroyed_at_call_correct.
+  destruct (In_dec preg_eq r pregs_destroyed_at_call) as [IN | NOTIN].
+  - rewrite undef_regs_same; auto.
+  - rewrite undef_regs_other; auto.
+Qed.
 
 (** Extract the values of the arguments of an external call.
     We exploit the calling conventions from module [Conventions], except that
@@ -1086,11 +1300,11 @@ Definition undef_caller_save_regs (rs: regset) : regset :=
 
 Inductive extcall_arg (rs: regset) (m: mem): loc -> val -> Prop :=
   | extcall_arg_reg: forall r,
-      extcall_arg rs m (R r) (rs (preg_of r))
+      extcall_arg rs m (R r) (rs # (preg_of r))
   | extcall_arg_stack: forall ofs q bofs v,
       bofs = Stacklayout.fe_ofs_arg + 4 * ofs ->
       Mem.loadv (chunk_of_quantity q) m
-                (Val.offset_ptr (rs (IR RSP)) (Ptrofs.repr bofs)) = Some v ->
+                (Val.offset_ptr (rs # (IR RSP)) (Ptrofs.repr bofs)) = Some v ->
       extcall_arg rs m (S Outgoing ofs q) v.
 
 Inductive extcall_arg_pair (rs: regset) (m: mem): rpair loc -> val -> Prop :=
@@ -1117,17 +1331,17 @@ Inductive state: Type :=
 Inductive step: state -> trace -> state -> Prop :=
   | exec_step_internal:
       forall b ofs f i rs m rs' m',
-      rs PC = Vptr b ofs ->
+      rs # PC = Vptr b ofs ->
       Genv.find_funct_ptr ge b = Some (Internal f) ->
       find_instr (Ptrofs.unsigned ofs) f.(fn_code) = Some i ->
       exec_instr f i rs m = Next rs' m' ->
       step (State rs m) E0 (State rs' m')
   | exec_step_builtin:
       forall b ofs f ef args res rs m vargs t vres rs' m',
-      rs PC = Vptr b ofs ->
+      rs # PC = Vptr b ofs ->
       Genv.find_funct_ptr ge b = Some (Internal f) ->
       find_instr (Ptrofs.unsigned ofs) f.(fn_code) = Some (Pbuiltin ef args res) ->
-      eval_builtin_args ge rs (rs RSP) m args vargs ->
+      eval_builtin_args ge (pregmap_read rs) (rs # RSP) m args vargs ->
       external_call ef ge vargs m t vres m' ->
       rs' = nextinstr_nf
              (set_res res vres
@@ -1135,11 +1349,11 @@ Inductive step: state -> trace -> state -> Prop :=
       step (State rs m) t (State rs' m')
   | exec_step_external:
       forall b ef args res rs m t rs' m',
-      rs PC = Vptr b Ptrofs.zero ->
+      rs # PC = Vptr b Ptrofs.zero ->
       Genv.find_funct_ptr ge b = Some (External ef) ->
       extcall_arguments rs m (ef_sig ef) args ->
       external_call ef ge args m t res m' ->
-      rs' = (set_pair (loc_external_result (ef_sig ef)) res (undef_caller_save_regs rs)) #PC <- (rs RA) ->
+      rs' = (set_pair (loc_external_result (ef_sig ef)) res (undef_caller_save_regs rs)) #PC <- (rs#RA) ->
       step (State rs m) t (State rs' m').
 
 End RELSEM.
@@ -1151,7 +1365,7 @@ Inductive initial_state (p: program): state -> Prop :=
       Genv.init_mem p = Some m0 ->
       let ge := Genv.globalenv p in
       let rs0 :=
-        (Pregmap.init Vundef)
+        Pregmap.init
         # PC <- (Genv.symbol_address ge p.(prog_main) Ptrofs.zero)
         # RA <- Vnullptr
         # RSP <- Vnullptr in
